test-suite/erasure_live_test.v
@@ -320,7 +320,6 @@ Require Import Coq.Arith.Peano_dec.
 Require Import Arith Wf.
 Program Fixpoint provedCopy (n:nat) {wf lt n} : nat :=
   match n with 0 => 0 | S k => S (provedCopy k) end.
-Next Obligation. eapply measure_wf, lt_wf. Qed. 
 Print Assumptions provedCopy.
 (* MetaCoq Quote Recursively Definition pCopy := provedCopy. program *)
 
